Types.v
@@ -28,37 +28,37 @@ Hint Constructors bvalue nvalue.
 Hint Unfold value.
 Hint Unfold extend.
 
-Reserved Notation "t1 '=>' t2" (at level 40).
+Reserved Notation "t1 '==>' t2" (at level 40).
 
 Inductive step : tm -> tm -> Prop :=
   | ST_IfTrue : forall t1 t2,
-      (tif ttrue t1 t2) => t1
+      (tif ttrue t1 t2) ==> t1
   | ST_IfFalse : forall t1 t2,
-      (tif tfalse t1 t2) => t2
+      (tif tfalse t1 t2) ==> t2
   | ST_If : forall t1 t1' t2 t3,
-      t1 => t1' ->
-      (tif t1 t2 t3) => (tif t1' t2 t3)
+      t1 ==> t1' ->
+      (tif t1 t2 t3) ==> (tif t1' t2 t3)
   | ST_Succ : forall t1 t1',
-      t1 => t1' ->
-      (tsucc t1) => (tsucc t1')
+      t1 ==> t1' ->
+      (tsucc t1) ==> (tsucc t1')
   | ST_PredZero :
-      (tpred tzero) => tzero
+      (tpred tzero) ==> tzero
   | ST_PredSucc : forall t1,
       nvalue t1 ->
-      (tpred (tsucc t1)) => t1
+      (tpred (tsucc t1)) ==> t1
   | ST_Pred : forall t1 t1',
-      t1 => t1' ->
-      (tpred t1) => (tpred t1')
+      t1 ==> t1' ->
+      (tpred t1) ==> (tpred t1')
   | ST_IszeroZero :
-      (tiszero tzero) => ttrue
+      (tiszero tzero) ==> ttrue
   | ST_IszeroSucc : forall t1,
        nvalue t1 ->
-      (tiszero (tsucc t1)) => tfalse
+      (tiszero (tsucc t1)) ==> tfalse
   | ST_Iszero : forall t1 t1',
-      t1 => t1' ->
-      (tiszero t1) => (tiszero t1')
+      t1 ==> t1' ->
+      (tiszero t1) ==> (tiszero t1')
 
-where "t1 '=>' t2" := (step t1 t2).
+where "t1 '==>' t2" := (step t1 t2).
 
 Tactic Notation "step_cases" tactic(first) ident(c) :=
   first;
@@ -93,34 +93,146 @@ Proof.
 
 Hint Resolve value_is_nf.
 
+Ltac find_replace :=
+  match goal with
+    H1 : ?T ==> ?T1, H2: ?T ==> ?T2 |- _ =>
+    (replace T2 with T1;eauto)
+  end.
+
+Ltac find_nvalcontra :=
+  match goal with
+    H1 : nvalue ?T , H2: ?T ==> ?T' |- _ =>
+    (assert(contra:False); eauto; try inversion contra; try eapply value_is_nf; eauto)
+  end.
+
 Theorem step_deterministic:
   deterministic step.
 Proof with eauto.
   intros t.
-  induction t; intros; inv H; inv H0; eauto.
-    inv H4.
-    inv H4.
-    inv H5.
-    inv H5.
-    replace t1'0 with t1'; eauto.
-    replace t1'0 with t1'; eauto.
-    inv H1.
-    inv H1. 
-    assert (contra:False); try inversion contra.
-      eapply value_is_nf; eauto.
-    inv H2. 
-    inv H2. 
-    assert (contra:False); try inversion contra.
-      eapply value_is_nf; eauto.
-    replace t1'0 with t1'; eauto.
-    inv H1.
-    inv H1. 
-    assert (contra:False); try inversion contra.
-      eapply value_is_nf; eauto.
-    inv H2. 
-    inv H2. 
-    assert (contra:False); try inversion contra.
-      eapply value_is_nf; eauto.
-    replace t1'0 with t1'; eauto.
+  induction t; intros; inv H; inv H0; eauto; 
+  try solve by inversion; try find_replace; 
+  try inversion H1; try inversion H2; subst;
+  try find_nvalcontra.
+  Qed.
+
+Inductive ty : Type :=
+  | TBool : ty
+  | TNat : ty.
+
+Reserved Notation "'|-' t '\in' T" (at level 40).
+
+Inductive has_type : tm -> ty -> Prop :=
+  | T_True : 
+       |- ttrue \in TBool
+  | T_False : 
+       |- tfalse \in TBool
+  | T_If : forall t1 t2 t3 T,
+       |- t1 \in TBool ->
+       |- t2 \in T ->
+       |- t3 \in T ->
+       |- tif t1 t2 t3 \in T
+  | T_Zero : 
+       |- tzero \in TNat
+  | T_Succ : forall t1,
+       |- t1 \in TNat ->
+       |- tsucc t1 \in TNat
+  | T_Pred : forall t1,
+       |- t1 \in TNat ->
+       |- tpred t1 \in TNat
+  | T_Iszero : forall t1,
+       |- t1 \in TNat ->
+       |- tiszero t1 \in TBool
+
+where "'|-' t '\in' T" := (has_type t T).
+
+Tactic Notation "has_type_cases" tactic(first) ident(c) :=
+  first;
+  [ Case_aux c "T_True" | Case_aux c "T_False" | Case_aux c "T_If"
+  | Case_aux c "T_Zero" | Case_aux c "T_Succ" | Case_aux c "T_Pred"
+  | Case_aux c "T_Iszero" ].
+
+Hint Constructors has_type.
+
+Example has_type_1 :
+  |- tif tfalse tzero (tsucc tzero) \in TNat.
+Proof.
+  auto. Qed.
+
+Example has_type_not :
+  ~ (|- tif tfalse tzero ttrue \in TBool).
+Proof. intros contra. inv contra. inv H4. Qed.
+
+Example succ_hastype_nat__hastype_nat : forall t,
+  |- tsucc t \in TNat ->
+  |- t \in TNat.
+Proof.
+  intros. inv H. assumption. Qed.
+
+Theorem progress : forall t T,
+  |- t \in T ->
+  value t \/ exists t', t ==> t'.
+Proof with auto.
+  intros t T HT.
+  has_type_cases (induction HT) Case...
+  Case "T_If".
+    right. inversion IHHT1; clear IHHT1.
+    SCase "t1 is a value". inversion H; clear H.
+      SSCase "t1 is a bvalue". inversion H0; clear H0.
+        SSSCase "t1 is ttrue".
+          exists t2...
+        SSSCase "t1 is tfalse". 
+          exists t3...
+      SSCase "t1 is an nvalue".
+        solve by inversion 2.  (* on H and HT1 *)
+    SCase "t1 can take a step".
+      inversion H as [t1' H1].
+      exists (tif t1' t2 t3)...
+  inv IHHT; inv H. inv H0; inv HT. left... right; eexists; eauto.
+  inv IHHT; inv H. inv H0; inv HT. inv H0; right; eexists; eauto. right; eexists; eauto.
+  inv IHHT; inv H. inv H0; inv HT. inv H0; right; eexists; eauto. right; eexists; eauto.
+  Qed.
+
+Lemma nvalue_isnat : forall t,
+  nvalue t -> |- t \in TNat.
+Proof.
+  intros; induction H; eauto.
+  Qed.
+
+Lemma bvalue_isbool : forall t,
+  bvalue t -> |- t \in TBool.
+Proof.
+  intros; induction H; eauto.
+  Qed.
+
+Hint Resolve nvalue_isnat.
+Hint Resolve bvalue_isbool.
+
+Theorem preservation : forall t t' T,
+  |- t \in T ->
+  t ==> t' ->
+  |- t' \in T.
+Proof with auto.
+  intros t t' T HT HE.
+  generalize dependent t'.
+  has_type_cases (induction HT) Case;
+         intros t' HE;
+         try (solve by inversion).
+    Case "T_If". inversion HE; subst.
+      SCase "ST_IFTrue". assumption.
+      SCase "ST_IfFalse". assumption.
+      SCase "ST_If". apply T_If; try assumption.
+        apply IHHT1; assumption.
+    inversion HE; subst; eauto.
+    inversion HE; subst; eauto.
+    inversion HE; subst; eauto.
+  Qed.
+
+Theorem preservation' : forall t t' T,
+  |- t \in T ->
+  t ==> t' ->
+  |- t' \in T.
+Proof with eauto.
+  intros. generalize dependent T.
+  induction H0; intros; inv H; eauto; inv H0; eauto.
   Qed.
 
